\exercise

The following linked list L is expressed as a sequence of pairs $(i, succ(i))$
and item 4 is the head of the list: $\mathcal{L} = \{ (1,6), (2,5), (3,0),
(4,2), (5,1), (6,3) \}$\footnote{We can assume the pair $(3, 0)$ represents the
last element of the list (with 0 as {\tt NULL} or ``no successor''), thus will
be represented from now on as $(3, 3)$, as in Prof. Ferragina's lecture notes.}.
Show all the steps needed to simulate the operation $succ(i) = succ(succ(i))$ of
the Pointer Jumping technique in the 2-levels model using a sequence of {\tt
sort} and {\tt scan}.

\solution

\autoref{fig:list1} shows the the initial state of the list $\mathcal{L}$. To
simulate the Pointer Jumping technique in the 2-levels model we first have to
store the list as \emph{triples} in the form of $\langle i, succ(i), rank(i)
\rangle$, initializing $rank(i) = 0$ if $succ(i) = i$ and $rank(i) = 1$
otherwise, as in \autoref{tab:list}. We store again the same list as
\emph{quadruples} such as $\langle i, succ(i), 0, 0 \rangle$, where the third
and fourth components of each tuple are temporary placeholders for the values of
$rank(succ(i))$ and $succ(succ(i))$, respectively. Then we proceed updating the
value of $rank(i)$ (in the triples) using a sequence of {\tt sort} and {\tt
scan} primitives, as follows:
%
\begin{align*}
  \text{\bf 1. }
  \begin{matrix}
    \langle 1, 6, 0, 0 \rangle \\
    \langle 2, 5, 0, 0 \rangle \\
    \langle 3, 3, 0, 0 \rangle \\
    \langle 4, 2, 0, 0 \rangle \\
    \langle 5, 1, 0, 0 \rangle \\
    \langle 6, 3, 0, 0 \rangle \\
  \end{matrix}
  \stackrel{\text{\tiny \tt sort}}{\longmapsto}
  \begin{matrix}
    \langle 5, 1, 0, 0 \rangle \\
    \langle 4, 2, 0, 0 \rangle \\
    \langle 3, 3, 0, 0 \rangle \\
    \langle 6, 3, 0, 0 \rangle \\
    \langle 2, 5, 0, 0 \rangle \\
    \langle 1, 6, 0, 0 \rangle \\
  \end{matrix}
  \stackrel{\text{\tiny \tt scan}}{\longmapsto}
  \begin{matrix}
    \langle 5, 1, 1, 6 \rangle \\
    \langle 4, 2, 1, 5 \rangle \\
    \langle 3, 3, 0, 3 \rangle \\
    \langle 6, 3, 0, 3 \rangle \\
    \langle 2, 5, 1, 1 \rangle \\
    \langle 1, 6, 1, 3 \rangle \\
  \end{matrix}
  \stackrel{\text{\tiny \tt sort}}{\longmapsto}
  \begin{matrix}
    \langle 1, 6, 1, 3 \rangle \\
    \langle 2, 5, 1, 1 \rangle \\
    \langle 3, 3, 0, 3 \rangle \\
    \langle 4, 2, 1, 5 \rangle \\
    \langle 5, 1, 1, 6 \rangle \\
    \langle 6, 3, 0, 3 \rangle \\
  \end{matrix}
  \stackrel{\text{\tiny \tt scan}}{\longmapsto}
  \begin{matrix}
    rank(1) + 1 = 2,\ succ(1) = 3 \\
    rank(2) + 1 = 2,\ succ(2) = 1 \\
    rank(3) + 0 = 0,\ succ(3) = 3 \\
    rank(4) + 1 = 2,\ succ(4) = 5 \\
    rank(5) + 1 = 2,\ succ(5) = 6 \\
    rank(6) + 0 = 1,\ succ(6) = 3 \\
  \end{matrix} \\[0.5em]
  \text{\bf 2. }
  \begin{matrix}
    \langle 1, 3, 0, 0 \rangle \\
    \langle 2, 1, 0, 0 \rangle \\
    \langle 3, 3, 0, 0 \rangle \\
    \langle 4, 5, 0, 0 \rangle \\
    \langle 5, 6, 0, 0 \rangle \\
    \langle 6, 3, 0, 0 \rangle \\
  \end{matrix}
  \stackrel{\text{\tiny \tt sort}}{\longmapsto}
  \begin{matrix}
    \langle 2, 1, 0, 0 \rangle \\
    \langle 1, 3, 0, 0 \rangle \\
    \langle 3, 3, 0, 0 \rangle \\
    \langle 6, 3, 0, 0 \rangle \\
    \langle 4, 5, 0, 0 \rangle \\
    \langle 5, 6, 0, 0 \rangle \\
  \end{matrix}
  \stackrel{\text{\tiny \tt scan}}{\longmapsto}
  \begin{matrix}
    \langle 2, 1, 2, 3 \rangle \\
    \langle 1, 3, 0, 3 \rangle \\
    \langle 3, 3, 0, 3 \rangle \\
    \langle 6, 3, 0, 3 \rangle \\
    \langle 4, 5, 2, 6 \rangle \\
    \langle 5, 6, 1, 3 \rangle \\
  \end{matrix}
  \stackrel{\text{\tiny \tt sort}}{\longmapsto}
  \begin{matrix}
    \langle 1, 3, 0, 3 \rangle \\
    \langle 2, 1, 2, 3 \rangle \\
    \langle 3, 3, 0, 3 \rangle \\
    \langle 4, 5, 2, 6 \rangle \\
    \langle 5, 6, 1, 3 \rangle \\
    \langle 6, 3, 0, 3 \rangle \\
  \end{matrix}
  \stackrel{\text{\tiny \tt scan}}{\longmapsto}
  \begin{matrix}
    rank(1) + 0 = 2,\ succ(1) = 3 \\
    rank(2) + 2 = 4,\ succ(2) = 3 \\
    rank(3) + 0 = 0,\ succ(3) = 3 \\
    rank(4) + 2 = 4,\ succ(4) = 6 \\
    rank(5) + 1 = 3,\ succ(5) = 3 \\
    rank(6) + 0 = 1,\ succ(6) = 3 \\
  \end{matrix} \\[0.5em]
  \text{\bf 3. }
  \begin{matrix}
    \langle 1, 3, 0, 0 \rangle \\
    \langle 2, 3, 0, 0 \rangle \\
    \langle 3, 3, 0, 0 \rangle \\
    \langle 4, 6, 0, 0 \rangle \\
    \langle 5, 3, 0, 0 \rangle \\
    \langle 6, 3, 0, 0 \rangle \\
  \end{matrix}
  \stackrel{\text{\tiny \tt sort}}{\longmapsto}
  \begin{matrix}
    \langle 1, 3, 0, 0 \rangle \\
    \langle 2, 3, 0, 0 \rangle \\
    \langle 3, 3, 0, 0 \rangle \\
    \langle 5, 3, 0, 0 \rangle \\
    \langle 6, 3, 0, 0 \rangle \\
    \langle 4, 6, 0, 0 \rangle \\
  \end{matrix}
  \stackrel{\text{\tiny \tt scan}}{\longmapsto}
  \begin{matrix}
    \langle 1, 3, 0, 3 \rangle \\
    \langle 2, 3, 0, 3 \rangle \\
    \langle 3, 3, 0, 3 \rangle \\
    \langle 5, 3, 0, 3 \rangle \\
    \langle 6, 3, 0, 3 \rangle \\
    \langle 4, 6, 1, 3 \rangle \\
  \end{matrix}
  \stackrel{\text{\tiny \tt sort}}{\longmapsto}
  \begin{matrix}
    \langle 1, 3, 0, 3 \rangle \\
    \langle 2, 3, 0, 3 \rangle \\
    \langle 3, 3, 0, 3 \rangle \\
    \langle 4, 6, 1, 3 \rangle \\
    \langle 5, 3, 0, 3 \rangle \\
    \langle 6, 3, 0, 3 \rangle \\
  \end{matrix}
  \stackrel{\text{\tiny \tt scan}}{\longmapsto}
  \begin{matrix}
    rank(1) + 0 = 2,\ succ(1) = 3 \\
    rank(2) + 0 = 4,\ succ(2) = 3 \\
    rank(3) + 0 = 0,\ succ(3) = 3 \\
    rank(4) + 1 = 5,\ succ(4) = 3 \\
    rank(5) + 0 = 3,\ succ(5) = 3 \\
    rank(6) + 0 = 1,\ succ(6) = 3 \\
  \end{matrix}
\end{align*}
%
Notice that, whenever we performa a {\tt sort}, we operate only on the
quadruples, while, whenever we perform a {\tt scan}, we operate both on the the
triples and on the quadruples, in parallel. Eventually, $succ(i)$ will have the
same value for each $i$, and the algorithm terminates. The final values of
$rank(i)$ stored in the triples will be the result of the algorithm and we may
throw away the contents of the quadruples.
%
\begin{table}[h]
  \centering
  \begin{tabular}{cc|cccccc}
                            & $i$       & 1 & 2 & 3 & 4 & 5 & 6 \\ \hline\hline
    \multirow{2}{*}{\bf 0.} & $succ(i)$ & 6 & 5 & 3 & 2 & 1 & 3 \\
                            & $rank(i)$ & 1 & 1 & 0 & 1 & 1 & 1 \\ \hline
    \multirow{2}{*}{\bf 1.} & $succ(i)$ & 3 & 1 & 3 & 5 & 6 & 3 \\
                            & $rank(i)$ & 2 & 2 & 0 & 2 & 2 & 1 \\ \hline
    \multirow{2}{*}{\bf 2.} & $succ(i)$ & 3 & 3 & 3 & 6 & 3 & 3 \\
                            & $rank(i)$ & 2 & 4 & 0 & 4 & 3 & 1 \\ \hline
    \multirow{2}{*}{\bf 3.} & $succ(i)$ & 3 & 3 & 3 & 3 & 3 & 3 \\
                            & $rank(i)$ & 2 & 4 & 0 & 5 & 3 & 1 \\ \hline
  \end{tabular}
  \caption{Memory representation of $\mathcal{L}$.}
  \label{tab:list}
\end{table}
%
\begin{figure} [h]
  \begin{subfigure}{\linewidth}
    \centering
    \begin{tikzpicture}[node distance=1.5cm, every node/.append style={draw,circle}]
      \node (a) {4};
      \node[right of=a] (b) {2};
      \node[right of=b] (c) {5};
      \node[right of=c] (d) {1};
      \node[right of=d] (e) {6};
      \node[right of=e] (f) {3};
      \draw[-latex] (a) -- (b);
      \draw[-latex] (b) -- (c);
      \draw[-latex] (c) -- (d);
      \draw[-latex] (d) -- (e);
      \draw[-latex] (e) -- (f);
      \path (f) edge[-latex, loop right] (f);
    \end{tikzpicture}
    \caption{Initial state.}
    \label{fig:list1}
  \end{subfigure} \vspace{1em} \\
  \begin{subfigure}{\linewidth}
    \centering
    \begin{tikzpicture}[node distance=1.5cm, every node/.append style={draw,circle}]
      \node (a) {4};
      \node[right of=a] (b) {2};
      \node[right of=b] (c) {5};
      \node[right of=c] (d) {1};
      \node[right of=d] (e) {6};
      \node[right of=e] (f) {3};
      \path (a) edge[-latex, out=-45, in=-135] (c);
      \path (b) edge[-latex, out=-45, in=-135] (d);
      \path (c) edge[-latex, out=-45, in=-135] (e);
      \path (d) edge[-latex, out=-45, in=-135] (f);
      \path (e) edge[-latex] (f);
      \path (f) edge[-latex, loop right] (f);
    \end{tikzpicture}
    \caption{First step.}
    \label{fig:list2}
  \end{subfigure} \vspace{1em} \\
  \begin{subfigure}{\linewidth}
    \centering
    \begin{tikzpicture}[node distance=1.5cm, every node/.append style={draw,circle}]
      \node (a) {4};
      \node[right of=a] (b) {2};
      \node[right of=b] (c) {5};
      \node[right of=c] (d) {1};
      \node[right of=d] (e) {6};
      \node[right of=e] (f) {3};
      \path (a) edge[-latex, out=-45, in=-135] (e);
      \path (b) edge[-latex, out=-45, in=-135] (f);
      \path (c) edge[-latex, out=-45, in=-135] (f);
      \path (d) edge[-latex, out=-45, in=-135] (f);
      \path (e) edge[-latex] (f);
      \path (f) edge[-latex, loop right] (f);
    \end{tikzpicture}
    \caption{Second step.}
    \label{fig:list2}
  \end{subfigure} \vspace{1em} \\
  \begin{subfigure}{\linewidth}
    \centering
    \begin{tikzpicture}[node distance=1.5cm, every node/.append style={draw,circle}]
      \node (a) {4};
      \node[right of=a] (b) {2};
      \node[right of=b] (c) {5};
      \node[right of=c] (d) {1};
      \node[right of=d] (e) {6};
      \node[right of=e] (f) {3};
      \path (a) edge[-latex, out=-45, in=-135] (f);
      \path (b) edge[-latex, out=-45, in=-135] (f);
      \path (c) edge[-latex, out=-45, in=-135] (f);
      \path (d) edge[-latex, out=-45, in=-135] (f);
      \path (e) edge[-latex] (f);
      \path (f) edge[-latex, loop right] (f);
    \end{tikzpicture}
    \caption{Third step.}
    \label{fig:list3}
  \end{subfigure}
  \caption{Graph representation of $\mathcal{L}$.}
  \label{fig:list}
\end{figure}
